Simple_Clause_Learning/Correct_Termination.thy
@@ -6,16 +6,15 @@ context scl begin
 
 lemma not_satisfiable_if_sound_state_conflict_bottom:
   assumes sound_S: "sound_state N \<beta> S" and conflict_S: "state_conflict S = Some ({#}, \<gamma>)"
-  shows "\<not> satisfiable (grounding_of_clss N)"
+  shows "\<not> satisfiable (grounding_of_clss (fset N))"
 proof -
-  from sound_S conflict_S have "N \<TTurnstile>\<G>e {{#}}"
+  from sound_S conflict_S have "fset N \<TTurnstile>\<G>e {{#}}"
     unfolding sound_state_def state_conflict_def by auto
   thus ?thesis by simp
 qed
 
 lemma propagate_if_conflict_follows_decide:
   assumes
-    fin_N: "finite N" and
     trail_lt_\<beta>: "trail_atoms_lt \<beta> S\<^sub>2" and
     no_conf: "\<nexists>S\<^sub>1. conflict N \<beta> S\<^sub>0 S\<^sub>1" and deci: "decide N \<beta> S\<^sub>0 S\<^sub>2" and conf: "conflict N \<beta> S\<^sub>2 S\<^sub>3"
   shows "\<exists>S\<^sub>4. propagate N \<beta> S\<^sub>0 S\<^sub>4"
@@ -23,7 +22,7 @@ proof -
   from deci obtain L \<gamma> \<Gamma> U where
     S\<^sub>0_def: "S\<^sub>0 = (\<Gamma>, U, None)" and
     S\<^sub>2_def: "S\<^sub>2 = (trail_decide \<Gamma> (L \<cdot>l \<gamma>), U, None)" and
-    "L \<in> \<Union> (set_mset ` N)" and
+    "L \<in> \<Union> (set_mset ` fset N)" and
     "is_ground_lit (L \<cdot>l \<gamma>)" and
     "\<not> trail_defined_lit \<Gamma> (L \<cdot>l \<gamma>)" and
     "atm_of L \<cdot>a \<gamma> \<prec>\<^sub>B \<beta>"
@@ -31,17 +30,16 @@ proof -
   
   from conf S\<^sub>2_def obtain D \<sigma> \<rho> \<sigma>\<^sub>\<rho> where
     S\<^sub>3_def: "S\<^sub>3 = (trail_decide \<Gamma> (L \<cdot>l \<gamma>), U, Some (D \<cdot> \<rho>, \<sigma>\<^sub>\<rho>))" and
-    D_in: "D \<in> N \<union> fset U" and
+    D_in: "D |\<in>| N |\<union>| U" and
     dom_\<sigma>_subset:"subst_domain \<sigma> \<subseteq> vars_cls D" and
     ground_D_\<sigma>: "is_ground_cls (D \<cdot> \<sigma>)" and
     tr_\<Gamma>_L_false_D: "trail_false_cls (trail_decide \<Gamma> (L \<cdot>l \<gamma>)) (D \<cdot> \<sigma>)" and
-    \<rho>_def: "\<rho> = renaming_wrt (N \<union> fset U \<union> clss_of_trail (trail_decide \<Gamma> (L \<cdot>l \<gamma>)))" and
+    \<rho>_def: "\<rho> = renaming_wrt (fset (N |\<union>| U |\<union>| clss_of_trail (trail_decide \<Gamma> (L \<cdot>l \<gamma>))))" and
     \<sigma>\<^sub>\<rho>_def: "\<sigma>\<^sub>\<rho> = adapt_subst_to_renaming \<rho> \<sigma>"
     by (elim conflict.cases) blast
 
   have ren_\<rho>: "is_renaming \<rho>"
-    unfolding \<rho>_def
-    by (rule is_renaming_renaming_wrt) (metis fin_N finite_fset finite_UnI finite_clss_of_trail)
+    unfolding \<rho>_def by (rule is_renaming_renaming_wrt[OF finite_fset])
 
   moreover have "vars_cls D \<subseteq> subst_domain \<sigma>"
     using ground_D_\<sigma> vars_cls_subset_subst_domain_if_grounding by blast
@@ -56,7 +54,7 @@ proof -
     unfolding \<open>D \<cdot> \<rho> \<cdot> \<sigma>\<^sub>\<rho> = D \<cdot> \<sigma>\<close> by (rule tr_\<Gamma>_L_false_D)
 
   moreover have "\<not> trail_false_cls \<Gamma> (D \<cdot> \<rho> \<cdot> \<sigma>\<^sub>\<rho>)"
-    using not_trail_false_ground_cls_if_no_conflict[OF fin_N no_conf] D_in
+    using not_trail_false_ground_cls_if_no_conflict[OF no_conf] D_in
     by (simp add: S\<^sub>0_def \<open>D \<cdot> \<rho> \<cdot> \<sigma>\<^sub>\<rho> = D \<cdot> \<sigma>\<close> ground_D_\<sigma>)
 
   ultimately have "- (L \<cdot>l \<gamma>) \<in># D \<cdot> \<rho> \<cdot> \<sigma>\<^sub>\<rho>"
@@ -234,13 +232,12 @@ definition conflict_minimal_subst_domain where
 
 lemma
   assumes
-    fin_N: "finite N" and
-    disj_N: "disjoint_vars_set N" and
+    disj_N: "disjoint_vars_set (fset N)" and
     regular_run: "(regular_scl N \<beta>)\<^sup>*\<^sup>* initial_state S" and
     no_more_regular_step: "\<nexists>S'. regular_scl N \<beta> S S'"
-  shows "\<not> satisfiable (grounding_of_clss N) \<and> (\<exists>\<gamma>. state_conflict S = Some ({#}, \<gamma>)) \<or>
-    satisfiable {C \<in> grounding_of_clss N. \<forall>L \<in># C. atm_of L \<prec>\<^sub>B \<beta>} \<and>
-      trail_true_clss (state_trail S) {C \<in> grounding_of_clss N. \<forall>L \<in># C. atm_of L \<prec>\<^sub>B \<beta>}"
+  shows "\<not> satisfiable (grounding_of_clss (fset N)) \<and> (\<exists>\<gamma>. state_conflict S = Some ({#}, \<gamma>)) \<or>
+    satisfiable {C \<in> grounding_of_clss (fset N). \<forall>L \<in># C. atm_of L \<prec>\<^sub>B \<beta>} \<and>
+      trail_true_clss (state_trail S) {C \<in> grounding_of_clss (fset N). \<forall>L \<in># C. atm_of L \<prec>\<^sub>B \<beta>}"
 proof -
   from regular_run have scl_run: "(scl N \<beta>)\<^sup>*\<^sup>* initial_state S"
   proof (rule mono_rtranclp[rule_format, rotated])
@@ -254,7 +251,7 @@ proof -
     using prod_cases3 by blast
 
   have sound_S: "sound_state N \<beta> S"
-    using regular_run_sound_state[OF regular_run] sound_initial_state[OF fin_N disj_N] by blast
+    using regular_run_sound_state[OF regular_run] sound_initial_state[OF disj_N] by blast
   hence sound_\<Gamma>: "sound_trail N \<Gamma>"
     by (simp add: S_def sound_state_def)
 
@@ -288,17 +285,17 @@ proof -
     proof (elim disjE exE conjE)
       assume no_new_decide: "\<nexists>S'. decide N \<beta> S S'"
 
-      have tr_true: "trail_true_clss \<Gamma> {C \<in> grounding_of_clss N. \<forall>L \<in># C. atm_of L \<prec>\<^sub>B \<beta>}"
+      have tr_true: "trail_true_clss \<Gamma> {C \<in> grounding_of_clss (fset N). \<forall>L \<in># C. atm_of L \<prec>\<^sub>B \<beta>}"
         unfolding trail_true_clss_def
       proof (rule ballI, unfold mem_Collect_eq, erule conjE)
-        fix C assume C_in: "C \<in> grounding_of_clss N" and C_lt_\<beta>: "\<forall>L \<in># C. atm_of L \<prec>\<^sub>B \<beta>"
+        fix C assume C_in: "C \<in> grounding_of_clss (fset N)" and C_lt_\<beta>: "\<forall>L \<in># C. atm_of L \<prec>\<^sub>B \<beta>"
 
         from C_in have "is_ground_cls C"
           by (rule grounding_ground)
 
-        from C_in obtain C' \<gamma> where C'_in: "C' \<in> N" and C_def: "C = C' \<cdot> \<gamma>"
-          using grounding_of_clss_def grounding_of_cls_def
-          by (smt (verit, del_insts) UN_iff mem_Collect_eq)
+        from C_in obtain C' \<gamma> where C'_in: "C' |\<in>| N" and C_def: "C = C' \<cdot> \<gamma>"
+          unfolding grounding_of_clss_def grounding_of_cls_def
+          by (smt (verit, ccfv_threshold) UN_iff mem_Collect_eq notin_fset)
 
         from no_new_decide have \<Gamma>_defined_C: "trail_defined_cls \<Gamma> C"
         proof (rule contrapos_np)
@@ -310,8 +307,9 @@ proof -
 
           have "decide N \<beta> (\<Gamma>, U, None) (trail_decide \<Gamma> (L' \<cdot>l \<gamma>), U, None)"
           proof (rule decideI)
-            show "L' \<in> \<Union> (set_mset ` N)"
-              using C'_in L'_in by blast
+            show "L' \<in> \<Union> (set_mset ` fset N)"
+              using C'_in L'_in
+              by (meson UN_I fmember.rep_eq)
           next
             show "is_ground_lit (L' \<cdot>l \<gamma>)"
               using L_in \<open>L = L' \<cdot>l \<gamma>\<close> \<open>is_ground_cls C\<close> is_ground_cls_def by blast
@@ -335,14 +333,14 @@ proof -
           assume "trail_false_cls \<Gamma> C"
 
           define \<rho> :: "'v \<Rightarrow> ('f, 'v) term" where
-            "\<rho> = renaming_wrt (N \<union> fset U \<union> clss_of_trail \<Gamma>)"
+            "\<rho> = renaming_wrt (fset (N |\<union>| U |\<union>| clss_of_trail \<Gamma>))"
 
           define \<gamma>\<^sub>\<rho> where
             "\<gamma>\<^sub>\<rho> = adapt_subst_to_renaming \<rho> (restrict_subst (vars_cls C') \<gamma>)"
 
           have "conflict N \<beta> (\<Gamma>, U, None) (\<Gamma>, U, Some (C' \<cdot> \<rho>, \<gamma>\<^sub>\<rho>))"
           proof (rule conflictI)
-            show "C' \<in> N \<union> fset U"
+            show "C' |\<in>| N |\<union>| U"
               using C'_in by simp
           next
             show "subst_domain (restrict_subst (vars_cls C') \<gamma>) \<subseteq> vars_cls C'"
@@ -361,13 +359,13 @@ proof -
           thus "trail_true_cls \<Gamma> C" ..
         qed
       qed
-      moreover have "satisfiable {C \<in> grounding_of_clss N. \<forall>L \<in># C. atm_of L \<prec>\<^sub>B \<beta>}"
+      moreover have "satisfiable {C \<in> grounding_of_clss (fset N). \<forall>L \<in># C. atm_of L \<prec>\<^sub>B \<beta>}"
         unfolding true_clss_def
       proof (intro exI ballI, unfold mem_Collect_eq, elim conjE)
         fix C
         have "trail_consistent \<Gamma>"
           using S_def trail_consistent by auto
-        show "C \<in> grounding_of_clss N \<Longrightarrow> \<forall>L \<in># C. atm_of L \<prec>\<^sub>B \<beta> \<Longrightarrow> trail_interp \<Gamma> \<TTurnstile> C"
+        show "C \<in> grounding_of_clss (fset N) \<Longrightarrow> \<forall>L \<in># C. atm_of L \<prec>\<^sub>B \<beta> \<Longrightarrow> trail_interp \<Gamma> \<TTurnstile> C"
           using tr_true[unfolded S_def, simplified]
           using trail_interp_cls_if_trail_true[OF \<open>trail_consistent \<Gamma>\<close>]
           by (simp add: trail_true_clss_def)
@@ -380,7 +378,7 @@ proof -
       moreover have "trail_atoms_lt \<beta> S'"
         by (rule decide_sound_state[OF deci sound_S, THEN trail_atoms_lt_if_sound_state])
       ultimately have "\<exists>S\<^sub>4. propagate N \<beta> S S\<^sub>4"
-        using propagate_if_conflict_follows_decide[OF fin_N _ no_new_conflict]
+        using propagate_if_conflict_follows_decide[OF _ no_new_conflict]
         by simp
       with no_new_propagate have False
         by blast
@@ -390,7 +388,7 @@ proof -
     case (Some Cl)
     then obtain C \<gamma> where u_def: "u = Some (C, \<gamma>)" by force
 
-    from sound_S have disj_vars_conflict: "\<forall>D \<in> N \<union> fset U \<union> clss_of_trail \<Gamma>. disjoint_vars C D"
+    from sound_S have disj_vars_conflict: "\<forall>D \<in> fset (N |\<union>| U |\<union>| clss_of_trail \<Gamma>). disjoint_vars C D"
       by (simp add: S_def u_def sound_state_def)
 
     from sound_S have domain_\<gamma>: "subst_domain \<gamma> \<subseteq> vars_cls C"
@@ -402,7 +400,7 @@ proof -
     show ?thesis
     proof (cases "C = {#}")
       case True
-      hence "\<not> satisfiable (grounding_of_clss N) \<and> (\<exists>\<gamma>. state_conflict S = Some ({#}, \<gamma>))"
+      hence "\<not> satisfiable (grounding_of_clss (fset N)) \<and> (\<exists>\<gamma>. state_conflict S = Some ({#}, \<gamma>))"
         using S_def u_def not_satisfiable_if_sound_state_conflict_bottom[OF sound_S] by simp
       thus ?thesis by simp
     next
@@ -418,7 +416,7 @@ proof -
         then obtain L n where \<Gamma>_def: "\<Gamma> = (L, n) # \<Gamma>'"
           by fastforce
 
-        from regular_run have mempty_not_in_N: "{#} \<notin> N"
+        from regular_run have mempty_not_in_N: "{#} |\<notin>| N"
           using C_not_empty mempty_not_in_initial_clauses_if_regular_run_reaches_non_empty_conflict
           unfolding S_def state_conflict_simp u_def option.inject
           by simp
@@ -447,8 +445,7 @@ proof -
               apply (erule conflict.cases)
               apply simp
               using mempty_not_in_N mempty_not_in_learned_S[unfolded S_def, simplified]
-              by (metis empty_not_add_mset finsertE not_trail_false_Nil(2) notin_fset
-                  subst_cls_empty_iff)
+              by (metis empty_not_add_mset finsertE not_trail_false_Nil(2) subst_cls_empty_iff)
 
             have "backtrack N \<beta> (\<Gamma>, U, Some (C' + {#K#}, \<gamma>)) ([], finsert (add_mset K C') U, None)"
               by (rule backtrackI[OF \<Gamma>_def' no_new_new_conflict])
@@ -476,7 +473,7 @@ proof -
               by (simp add: S_def trail_groundings_def 1 trail_propagate_def)
 
             define \<rho> :: "'v \<Rightarrow> ('f, 'v) Term.term" where
-              "\<rho> = renaming_wrt (N \<union> fset U \<union> clss_of_trail \<Gamma> \<union> {C' + {#K#}})"
+              "\<rho> = renaming_wrt (fset (N |\<union>| U |\<union>| clss_of_trail \<Gamma> |\<union>| {|C' + {#K#}|}))"
 
             have *: "vars_cls (add_mset L' D) \<inter> vars_cls (add_mset K C') = {}"
               using disj_vars_conflict[unfolded C_def 1]
